Specify decl-intersection, give an intersection function, prove it correct. Spec is very nice and concise, proofs are not, but this is due to bad coding style, not to bad infrastructure.

RecordsNoLib.v
@@ -91,11 +91,16 @@ Parameter B : Type.
 Parameter key: B -> K.
 Parameter value: B -> V. 
 Axiom eq_key_dec: forall k1 k2: K, {k1 = k2} + {k1 <> k2}.
+Axiom key_val_eq_eq: forall b1 b2, key b1 = key b2 -> value b1 = value b2 -> b1 = b2.
 End EnvParams.
+
+Ltac inv H := inversion H; clear H; subst.
 
 (* General environment *)
 Module Env (params: EnvParams).
 Import params.
+Definition key := key.
+Definition value := value.
 Definition t := list B.
 Definition map: (B -> B) -> t -> t := (@List.map B B).
 Fixpoint get(k: K)(E: t): option V := match E with
@@ -104,6 +109,108 @@ Fixpoint get(k: K)(E: t): option V := match E with
   end.
 Definition binds(k: K)(v: V)(E: t): Prop := (get k E = Some v).
 Definition unbound(k: K)(E: t): Prop := (get k E = None).
+Lemma binds_empty_inv : forall k v, binds k v nil -> False.
+Proof.
+  intros. unfold binds, get in H. discriminate H.
+Qed.
+Lemma map_head: forall (E: t) (b: B) (f: B -> B), map f (E ;; b) = (map f E) ;; (f b).
+Proof.
+  intros. destruct E as [|a E].
+  + unfold map. unfold List.map. reflexivity.
+  + unfold map. remember (E ;; a) as L. unfold List.map. reflexivity.
+Qed.
+Lemma concat_cons_assoc: forall (E1: t) (E2: t) (b: B), E1 & (E2 ;; b) = (E1 & E2) ;; b.
+Proof.
+  intros. simpl. reflexivity.
+Qed.
+Lemma binds_unbound_inv: forall E b, unbound (key b) (E ;; b) -> False.
+Proof.
+  intros. unfold unbound in H. simpl in H. destruct (eq_key_dec (key b) (key b)).
+  + discriminate H.
+  + apply n. reflexivity.
+Qed.
+Lemma unbound_cons_inv: forall E k b, unbound k (E ;; b) -> unbound k E.
+Proof.
+  intros. unfold unbound in H. unfold get in H. destruct (eq_key_dec k (key b)).
+  + inversion H.
+  + fold get in H. unfold unbound. assumption.
+Qed.
+Lemma binds_push_eq_inv: forall E a b,
+  binds (key a) (value b) (E ;; a) -> value a = value b.
+Proof.
+  intros. unfold binds, get in H. destruct (eq_key_dec (key a) (key a)).
+  + inversion H. reflexivity.
+  + contradiction n. reflexivity.
+Qed.
+Lemma binds_binding_inv: forall k v E, binds k v E -> exists b, key b = k /\ value b = v.
+Proof.
+  intros k v E. induction E; intros.
+  + exfalso. apply (@binds_empty_inv _ _ H).
+  + unfold binds, get in H. fold get in H. destruct (eq_key_dec k (key a)).
+    - inversion H. rewrite -> H1. exists a. symmetry in e. split; assumption.
+    - unfold binds in IHE. apply IHE. assumption.
+Qed.
+Lemma binds_map: forall b (f : B -> B) E,
+  (forall a, key (f a) = key a) ->
+  binds (key b) (value b) E -> 
+  binds (key (f b)) (value (f b)) (map f E).
+Proof.
+  intros. induction E.
+  + exfalso. apply (@binds_empty_inv _ _ H0).
+  + simpl. unfold binds, get. rewrite -> (H a). rewrite -> (H b).
+    unfold binds, get in H0. destruct (eq_key_dec (key b) (key a)).
+    - inv H0. do 3 f_equal. symmetry in e. apply key_val_eq_eq; assumption.
+    - fold get. fold get in H0. unfold binds in IHE. 
+      rewrite -> (H b) in IHE. apply (IHE H0).
+Qed.
+Lemma unbound_map: forall k (f : B -> B) E,
+  (forall a, key (f a) = key a) ->
+  unbound k E -> 
+  unbound k (map f E).
+Proof.
+  intros. induction E.
+  + simpl. assumption.
+  + simpl. unfold unbound, get. fold get. rewrite -> (H a).
+    destruct (eq_key_dec k (key a)).
+    - exfalso. rewrite -> e in H0. apply (binds_unbound_inv E a H0).
+    - unfold unbound in IHE. apply IHE. apply unbound_cons_inv in H0.
+      unfold unbound in H0. assumption.
+Qed.
+Lemma binds_concat_right : forall k v E1 E2,
+  binds k v E2 ->
+  binds k v (E1 & E2).
+Proof.
+  intros. induction E2.
+  + exfalso. apply (@binds_empty_inv _ _ H).
+  + rewrite -> concat_cons_assoc. unfold binds, get. unfold binds, get in H.
+    destruct (eq_key_dec k (key a)).
+    - assumption.
+    - fold get in *. unfold binds in IHE2. apply IHE2. assumption.
+Qed.
+Lemma binds_concat_left_inv : forall k v E1 E2,
+  binds k v (E1 & E2) ->
+  unbound k E2 ->
+  binds k v E1.
+Proof.
+  intros. induction E2.
+  + simpl in H. assumption.
+  + rewrite -> concat_cons_assoc in H. unfold binds, get in H. fold get in H.
+    destruct (eq_key_dec k (key a)).
+    - exfalso. rewrite -> e in H0. apply (binds_unbound_inv E2 a H0).
+    - apply IHE2. unfold binds. assumption. apply (@unbound_cons_inv E2 k a H0).
+Qed.
+Lemma binds_concat_left : forall k v E1 E2,
+  binds k v E1 ->
+  unbound k E2 ->
+  binds k v (E1 & E2).
+Proof.
+  intros. induction E2.
+  + simpl. assumption.
+  + rewrite -> concat_cons_assoc. unfold binds, get. fold get.
+    destruct (eq_key_dec k (key a)).
+    - exfalso. rewrite -> e in H0. apply (binds_unbound_inv E2 a H0).
+    - unfold binds in IHE2. apply IHE2. apply (@unbound_cons_inv E2 k a H0).
+Qed.
 End Env.
 
 (* Module decs: For lists of declarations: [list ndec] or [label => dec] *)
@@ -120,6 +227,14 @@ Definition value(d: ndec): dec := match d with
 | ndec_mtd n T U => dec_mtd T U
 end.
 Definition eq_key_dec := eq_label_dec.
+Lemma key_val_eq_eq: forall b1 b2, key b1 = key b2 -> value b1 = value b2 -> b1 = b2.
+Proof.
+  intros. destruct b1, b2.
+  + inv H. inv H0. reflexivity.
+  + inv H.
+  + inv H.
+  + inv H. inv H0. reflexivity.
+Qed.
 End decsParams.
 Module decs := Env(decsParams).
 
@@ -137,6 +252,14 @@ Definition value(i: nini): ini := match i with
 | nini_mtd n T e => ini_mtd T e
 end.
 Definition eq_key_dec := eq_label_dec.
+Lemma key_val_eq_eq: forall b1 b2, key b1 = key b2 -> value b1 = value b2 -> b1 = b2.
+Proof.
+  intros. destruct b1, b2.
+  + inv H. inv H0. reflexivity.
+  + inv H.
+  + inv H.
+  + inv H. inv H0. reflexivity.
+Qed.
 End inisParams.
 Module inis := Env(inisParams).
 
@@ -148,6 +271,10 @@ Definition B := (var * typ)%type.
 Definition key := @fst var typ.
 Definition value := @snd var typ.
 Definition eq_key_dec := eq_nat_dec.
+Lemma key_val_eq_eq: forall b1 b2, key b1 = key b2 -> value b1 = value b2 -> b1 = b2.
+Proof.
+  intros. destruct b1, b2. unfold key, fst, value, snd in *. subst. reflexivity.
+Qed.
 End tenvParams.
 Module tenv := Env(tenvParams).
 
@@ -159,8 +286,360 @@ Definition B := (var * inis.t)%type.
 Definition key := @fst var inis.t.
 Definition value := @snd var inis.t.
 Definition eq_key_dec := eq_nat_dec.
+Lemma key_val_eq_eq: forall b1 b2, key b1 = key b2 -> value b1 = value b2 -> b1 = b2.
+Proof.
+  intros. destruct b1, b2. unfold key, fst, value, snd in *. subst. reflexivity.
+Qed.
 End venvParams.
 Module venv := Env(venvParams).
+
+Module Type IntersectionPreview.
+
+(* Will be part of syntax: *)
+Parameter t_and: typ -> typ -> typ.
+Parameter t_or:  typ -> typ -> typ.
+
+(* Left as an exercise for the reader ;-) We define intersection by the spec below. *)
+Parameter intersect: decs.t -> decs.t -> decs.t.
+
+Axiom intersect_spec_1: forall l d ds1 ds2,
+  decs.binds   l d ds1 ->
+  decs.unbound l ds2 ->
+  decs.binds   l d (intersect ds1 ds2).
+
+Axiom intersect_spec_2: forall l d ds1 ds2,
+  decs.unbound l ds1 ->
+  decs.binds   l d ds2 ->
+  decs.binds   l d (intersect ds1 ds2).
+
+Axiom intersect_spec_12_fld: forall n T1 T2 ds1 ds2,
+  decs.binds (label_fld n) (dec_fld T1) ds1 ->
+  decs.binds (label_fld n) (dec_fld T2) ds2 ->
+  decs.binds (label_fld n) (dec_fld (t_and T1 T2)) (intersect ds1 ds2).
+
+Axiom intersect_spec_12_mtd: forall n S1 T1 S2 T2 ds1 ds2,
+  decs.binds (label_mtd n) (dec_mtd S1 T1) ds1 ->
+  decs.binds (label_mtd n) (dec_mtd S2 T2) ds2 ->
+  decs.binds (label_mtd n) (dec_mtd (t_or S1 S2) (t_and T1 T2)) (intersect ds1 ds2).
+
+End IntersectionPreview.
+
+(* Exercise: Give any implementation of `intersect`, and prove that it satisfies
+   the specification. Happy hacking! ;-) *)
+Module IntersectionPreviewImpl <: IntersectionPreview.
+
+(* Will be part of syntax: *)
+Parameter t_and: typ -> typ -> typ.
+Parameter t_or:  typ -> typ -> typ.
+
+Fixpoint get_fld(n: nat)(ds: decs.t): option typ := match ds with
+  | nil => None
+  | tail ;; d => match d with
+      | ndec_fld m T => if eq_nat_dec n m then Some T else get_fld n tail
+      | _ => get_fld n tail
+      end
+  end.
+(*
+Lemma get_fld_spec: forall n ds, decs.get (label_fld n) ds = dec_fld (get_fld n ds).
+Proof.
+*)
+
+Fixpoint refine_dec(d1: ndec)(ds2: decs.t): ndec := match ds2 with
+| nil => d1
+| tail2 ;; d2 => match d1, d2 with
+    | ndec_fld n1 T1   , ndec_fld n2 T2    => if eq_nat_dec n1 n2
+                                              then ndec_fld n1 (t_and T1 T2) 
+                                              else refine_dec d1 tail2
+    | ndec_mtd n1 T1 S1, ndec_mtd n2 T2 S2 => if eq_nat_dec n1 n2
+                                              then ndec_mtd n1 (t_or T1 T2) (t_and S1 S2) 
+                                              else refine_dec d1 tail2
+    | _, _ => refine_dec d1 tail2
+    end
+end.
+
+Ltac destruct_matchee :=
+  match goal with
+  | [ Hm: match ?e1 with _ => _ end = _ |- _ ]  => 
+      remember e1 as mExpr; destruct mExpr
+  | [ Hm: if ?e1 then _ else _ = _ |- _ ]  => 
+      remember e1 as mExpr; destruct mExpr
+  end.
+
+Lemma refine_dec_spec_fld: forall ds2 n T1 T2,
+  decs.binds (label_fld n) (dec_fld T2) ds2 ->
+  (refine_dec (ndec_fld n T1) ds2) = (ndec_fld n (t_and T1 T2)).
+Proof. 
+  intro ds2. induction ds2; intros.
+  + apply decs.binds_empty_inv in H. contradiction H.
+  + unfold decs.binds in H. unfold decs.get in H. unfold decs.key, decsParams.key in H.
+    destruct_matchee.
+    - inv H. unfold decs.value, decsParams.value in H1. destruct a eqn: Heqa.
+      * inv H1. inversion e. subst. simpl. destruct (eq_nat_dec n0 n0). reflexivity.
+        contradiction n. reflexivity.
+      * inv H1.
+    - simpl. destruct a eqn: Heqa. 
+      * assert (Hnn: n <> n1). unfold not in *. intro. apply n0. f_equal. assumption.
+        destruct (eq_nat_dec n n1). contradiction Hnn.
+        apply IHds2. unfold decs.binds, decs.get. unfold decs.key, decsParams.key.
+        assumption.
+      * apply IHds2. unfold decs.binds, decs.get. unfold decs.key, decsParams.key.
+        assumption.
+Qed.
+
+Lemma refine_dec_spec_mtd: forall ds2 n T1 S1 T2 S2,
+  decs.binds (label_mtd n) (dec_mtd T2 S2) ds2 ->
+  (refine_dec (ndec_mtd n T1 S1) ds2) = (ndec_mtd n (t_or T1 T2) (t_and S1 S2)).
+Proof. 
+  intro ds2. induction ds2; intros.
+  + apply decs.binds_empty_inv in H. contradiction H.
+  + unfold decs.binds in H. unfold decs.get in H. unfold decs.key, decsParams.key in H.
+    destruct_matchee.
+    - inv H. unfold decs.value, decsParams.value in H1. destruct a eqn: Heqa.
+      * inv H1.
+      * inv H1. inversion e. subst. simpl. destruct (eq_nat_dec n0 n0). reflexivity.
+        contradiction n. reflexivity.
+    - simpl. destruct a eqn: Heqa. 
+      * apply IHds2. unfold decs.binds, decs.get. unfold decs.key, decsParams.key.
+        assumption.
+      * assert (Hnn: n <> n1). unfold not in *. intro. apply n0. f_equal. assumption.
+        destruct (eq_nat_dec n n1). contradiction Hnn.
+        apply IHds2. unfold decs.binds, decs.get. unfold decs.key, decsParams.key.
+        assumption.
+Qed.
+
+Lemma refine_dec_spec_label: forall d1 ds2, decs.key d1 = decs.key (refine_dec d1 ds2).
+Proof.
+  intros.
+  induction ds2.
+  + simpl. reflexivity.
+  + unfold decs.key, decsParams.key. unfold refine_dec. destruct a; destruct d1.
+    - destruct (eq_nat_dec n0 n).
+      * simpl. reflexivity.
+      * fold refine_dec. unfold decs.key, decsParams.key in IHds2.
+        rewrite <- IHds2. reflexivity.
+    - fold refine_dec. unfold decs.key, decsParams.key in IHds2.
+        rewrite <- IHds2. reflexivity.
+    - fold refine_dec. unfold decs.key, decsParams.key in IHds2.
+        rewrite <- IHds2. reflexivity.
+    - destruct (eq_nat_dec n0 n).
+      * simpl. reflexivity.
+      * fold refine_dec. unfold decs.key, decsParams.key in IHds2.
+        rewrite <- IHds2. reflexivity.
+Qed.
+
+Lemma refine_dec_spec_unbound: forall d1 ds2, 
+  decs.unbound (decs.key d1) ds2 ->
+  decs.value (refine_dec d1 ds2) = decs.value d1.
+Proof.
+  intros.
+  induction ds2.
+  + simpl. reflexivity.
+  + unfold decs.key, decsParams.key. unfold refine_dec. destruct a; destruct d1.
+    - destruct (eq_nat_dec n0 n) eqn: Hn0ndec.
+      * subst. 
+        assert (Hkeq: (decs.key (ndec_fld n t0)) = (decs.key (ndec_fld n t)))
+          by reflexivity.
+        rewrite -> Hkeq in H.
+        exfalso. apply (decs.binds_unbound_inv _ _ H).
+      * fold refine_dec. apply IHds2.
+        inv H. unfold decsParams.eq_key_dec in H1. 
+        destruct (eq_label_dec (label_fld n0) (label_fld n)).
+        { inv e. contradiction n1. reflexivity. }
+        { unfold decs.unbound. unfold decs.key, decsParams.key. assumption. }
+    - fold refine_dec. unfold decs.key, decsParams.key in *.
+      apply decs.unbound_cons_inv in H. apply (IHds2 H).
+    - fold refine_dec. unfold decs.key, decsParams.key in *.
+      apply decs.unbound_cons_inv in H. apply (IHds2 H).
+    - destruct (eq_nat_dec n0 n) eqn: Hn0ndec.
+      * subst. 
+        assert (Hkeq: (decs.key (ndec_mtd n t1 t2)) = (decs.key (ndec_mtd n t t0)))
+          by reflexivity.
+        rewrite -> Hkeq in H.
+        exfalso. apply (decs.binds_unbound_inv _ _ H).
+      * fold refine_dec. apply IHds2.
+        inv H. unfold decsParams.eq_key_dec in H1. 
+        destruct (eq_label_dec (label_mtd n0) (label_mtd n)).
+        { inv e. contradiction n1. reflexivity. }
+        { unfold decs.unbound. unfold decs.key, decsParams.key. assumption. }
+Qed.
+
+Definition refine_decs(ds1: decs.t)(ds2: decs.t): decs.t := 
+  decs.map (fun d1 => refine_dec d1 ds2) ds1.
+
+Lemma refine_decs_spec_unbound: forall l d ds1 ds2,
+  decs.binds   l d ds1 ->
+  decs.unbound l ds2 ->
+  decs.binds   l d (refine_decs ds1 ds2).
+Proof.
+  intros. unfold refine_decs. unfold decs.map.  
+  assert (Hex: exists nd, decs.key nd = l /\ decs.value nd = d).
+    apply (@decs.binds_binding_inv l d ds1 H).
+  destruct Hex as [nd [Hl Hd]]. subst.
+  remember (fun d1 : decsParams.B => refine_dec d1 ds2) as f.
+  assert (Hk: (decs.key nd) = decs.key (f nd)).
+    subst. apply (refine_dec_spec_label nd ds2).
+  rewrite -> Hk.
+  assert (Hv: (decs.value nd) = decs.value (f nd)).
+    subst. symmetry. apply (refine_dec_spec_unbound _ _ H0).
+  rewrite -> Hv.
+  apply decs.binds_map. 
+    intro. rewrite -> Heqf. symmetry. apply refine_dec_spec_label.
+    assumption.
+Qed.
+
+Lemma refine_decs_spec_unbound_preserved: forall l ds1 ds2,
+  decs.unbound l ds1 ->
+  decs.unbound l (refine_decs ds1 ds2).
+Proof.
+  intros. unfold refine_decs. remember (fun d1 : decsParams.B => refine_dec d1 ds2) as f.
+  refine (decs.unbound_map l f ds1 _ H).
+  subst. intro. symmetry. apply refine_dec_spec_label.
+Qed.
+
+Lemma refine_decs_spec_fld: forall n ds1 ds2 T1 T2,
+  decs.binds (label_fld n) (dec_fld T1) ds1 ->
+  decs.binds (label_fld n) (dec_fld T2) ds2 ->
+  decs.binds (label_fld n) (dec_fld (t_and T1 T2)) (refine_decs ds1 ds2).
+Proof.
+  intros n ds1 ds2 T1 T2 H. induction ds1; intros.
+  + apply decs.binds_empty_inv in H. contradiction H.
+  + unfold decs.binds, decs.get in H. destruct a eqn: Heqa.
+    - fold decs.get in H. unfold decs.key, decsParams.key in H.
+      destruct (decsParams.eq_key_dec (label_fld n) (label_fld n0)).
+      * inv H. inv e.
+        unfold decs.binds, decs.get. simpl. fold decs.get. 
+        rewrite <- (@refine_dec_spec_label (ndec_fld n0 T1) ds2).
+        unfold decs.key, decsParams.key.
+        destruct (decsParams.eq_key_dec (label_fld n0) (label_fld n0)). {
+          f_equal. rewrite -> (@refine_dec_spec_fld ds2 n0 T1 T2 H0).
+          simpl. reflexivity. 
+        } { contradiction n. reflexivity. }
+      * assert (Hnn: n <> n0). unfold not in *. intro. apply n1. f_equal. assumption.
+        unfold decs.binds, decs.get. simpl. fold decs.get. 
+        rewrite <- (@refine_dec_spec_label (ndec_fld n0 t) ds2).
+        unfold decs.key, decsParams.key.
+        destruct (decsParams.eq_key_dec (label_fld n) (label_fld n0)). {
+          inv e. contradiction Hnn. reflexivity.
+        } {
+          unfold decs.binds in *. apply IHds1; assumption.
+        }
+    - fold decs.get in H. unfold decs.key, decsParams.key in H.
+      destruct (decsParams.eq_key_dec (label_fld n) (label_fld n0)).
+      * inv H. inv e.
+        unfold decs.binds, decs.get. simpl. fold decs.get.
+        rewrite <- (@refine_dec_spec_label (ndec_mtd n0 t t0) ds2).
+        unfold decs.key, decsParams.key.
+        destruct (decsParams.eq_key_dec (label_fld n0) (label_mtd n0)). {
+          inv H2.
+        } {
+          unfold decs.binds in *. apply IHds1; assumption.
+        }
+      * assert (Hnn: n <> n0). unfold not in *. intro. apply n1. f_equal. assumption.
+        unfold decs.binds, decs.get. simpl. fold decs.get. 
+        rewrite <- (@refine_dec_spec_label (ndec_mtd n0 t t0) ds2).
+        unfold decs.key, decsParams.key.
+        destruct (decsParams.eq_key_dec (label_fld n) (label_fld n0)). {
+          inv e. contradiction Hnn. reflexivity.
+        } {
+          destruct (decsParams.eq_key_dec (label_fld n) (label_mtd n0)).
+          + inv e.
+          + unfold decs.binds in *. apply IHds1; assumption.
+        }
+Qed.
+
+Lemma refine_decs_spec_mtd: forall n ds1 ds2 T1 S1 T2 S2,
+  decs.binds (label_mtd n) (dec_mtd T1 S1) ds1 ->
+  decs.binds (label_mtd n) (dec_mtd T2 S2) ds2 ->
+  decs.binds (label_mtd n) (dec_mtd (t_or T1 T2) (t_and S1 S2)) (refine_decs ds1 ds2).
+Proof.
+  intros n ds1 ds2 T1 S1 T2 S2 H. induction ds1; intros.
+  + apply decs.binds_empty_inv in H. contradiction H.
+  + unfold decs.binds, decs.get in H. destruct a eqn: Heqa.
+    - fold decs.get in H. unfold decs.key, decsParams.key in H.
+      destruct (decsParams.eq_key_dec (label_mtd n) (label_mtd n0)).
+      * inv H. inv e.
+        unfold decs.binds, decs.get. simpl. fold decs.get.
+        rewrite <- (@refine_dec_spec_label (ndec_fld n0 t) ds2).
+        unfold decs.key, decsParams.key.
+        destruct (decsParams.eq_key_dec (label_mtd n0) (label_fld n0)). {
+          inv H2.
+        } {
+          unfold decs.binds in *. apply IHds1; assumption.
+        }
+      * assert (Hnn: n <> n0). unfold not in *. intro. apply n1. f_equal. assumption.
+        unfold decs.binds, decs.get. simpl. fold decs.get. 
+        rewrite <- (@refine_dec_spec_label (ndec_fld n0 t) ds2).
+        unfold decs.key, decsParams.key.
+        destruct (decsParams.eq_key_dec (label_mtd n) (label_mtd n0)). {
+          inv e. contradiction Hnn. reflexivity.
+        } {
+          destruct (decsParams.eq_key_dec (label_mtd n) (label_fld n0)).
+          + inv e.
+          + unfold decs.binds in *. apply IHds1; assumption.
+        }
+    - fold decs.get in H. unfold decs.key, decsParams.key in H.
+      destruct (decsParams.eq_key_dec (label_mtd n) (label_mtd n0)).
+      * inv H. inv e.
+        unfold decs.binds, decs.get. simpl. fold decs.get. 
+        rewrite <- (@refine_dec_spec_label (ndec_mtd n0 T1 S1) ds2).
+        unfold decs.key, decsParams.key.
+        destruct (decsParams.eq_key_dec (label_mtd n0) (label_mtd n0)). {
+          f_equal. rewrite -> (@refine_dec_spec_mtd ds2 n0 T1 S1 T2 S2 H0).
+          simpl. reflexivity. 
+        } { contradiction n. reflexivity. }
+      * assert (Hnn: n <> n0). unfold not in *. intro. apply n1. f_equal. assumption.
+        unfold decs.binds, decs.get. simpl. fold decs.get. 
+        rewrite <- (@refine_dec_spec_label (ndec_mtd n0 t t0) ds2).
+        unfold decs.key, decsParams.key.
+        destruct (decsParams.eq_key_dec (label_mtd n) (label_mtd n0)). {
+          inv e. contradiction Hnn. reflexivity.
+        } {
+          unfold decs.binds in *. apply IHds1; assumption.
+        } 
+Qed.
+
+
+(* refined decs shadow the outdated decs of ds2 *)
+Definition intersect(ds1 ds2: decs.t): decs.t := ds2 & (refine_decs ds1 ds2).
+
+Lemma intersect_spec_1: forall l d ds1 ds2,
+  decs.binds   l d ds1 ->
+  decs.unbound l ds2 ->
+  decs.binds   l d (intersect ds1 ds2).
+Proof.
+  intros. unfold intersect. apply decs.binds_concat_right.
+  apply refine_decs_spec_unbound; assumption.
+Qed.
+
+Lemma intersect_spec_2: forall l d ds1 ds2,
+  decs.unbound l ds1 ->
+  decs.binds   l d ds2 ->
+  decs.binds   l d (intersect ds1 ds2).
+Proof.
+  intros. unfold intersect.
+  apply (@decs.binds_concat_left l d ds2 (refine_decs ds1 ds2) H0). 
+  apply (@refine_decs_spec_unbound_preserved l ds1 ds2 H). 
+Qed.
+
+Lemma intersect_spec_12_fld: forall n T1 T2 ds1 ds2,
+  decs.binds (label_fld n) (dec_fld T1) ds1 ->
+  decs.binds (label_fld n) (dec_fld T2) ds2 ->
+  decs.binds (label_fld n) (dec_fld (t_and T1 T2)) (intersect ds1 ds2).
+Proof.
+  intros. unfold intersect. apply decs.binds_concat_right.
+  apply refine_decs_spec_fld; assumption.
+Qed.
+
+Lemma intersect_spec_12_mtd: forall n S1 T1 S2 T2 ds1 ds2,
+  decs.binds (label_mtd n) (dec_mtd S1 T1) ds1 ->
+  decs.binds (label_mtd n) (dec_mtd S2 T2) ds2 ->
+  decs.binds (label_mtd n) (dec_mtd (t_or S1 S2) (t_and T1 T2)) (intersect ds1 ds2).
+Proof.
+  intros. unfold intersect. apply decs.binds_concat_right.
+  apply refine_decs_spec_mtd; assumption.
+Qed.
+
+End IntersectionPreviewImpl.
 
 (* ... opening ...
    replaces in some syntax a bound variable with dangling index (k) by a free variable x
